\section{Subspaces}

\begin{mydef}
  A subset $U$ of $V$ ($U \subseteq V$) is called a ``subspace" of $V$ if $U$ is also a vector space with the same additive identity, addition, and scalar multiplication as on $V$.
\end{mydef}

\begin{thm}
  A subset $U$ of $V$ is a subspace of $V$ $\iff$ $U$ satisfies the following three conditions:
  \begin{itemize}
    \item \bfemph{Additive identity:}
    $0 \in U$
    \item \bfemph{Closed under addition:}
    $u,w \in U \implies u+w \in U$
    \item \bfemph{Closed under scalar multiplication:}
    $a \in \myF$ and $u \in U \implies au \in U$
  \end{itemize}
  The additive identity condition above could be replaced by the condition that $U$ is nonempty (because then taking $u \in U$ and multiplying it by $0$ would imply that $0\in U$).
\end{thm}


%\textbf{1.34} $U\subseteq V$ is a subspace of $V$ $\iff$
%\begin{itemize}
%	\item additive identity: $0 \in U$
%	\item closed under addition: $u,w\in U \implies u+w \in U$
%	\item closed under scalar multiplication: $a \in \myF$ and $u\in U$ $\implies$ $au \in U$
%\end{itemize}

\subsection{Sum of Subspaces}

\setcounter{thm}{35}

\begin{mydef}
  $V_1 + \cdots + V_m :\equiv \{v_1 + \cdots + v_m \mid v_1 \in V_1, \, \dots \, , v_m \in V_m \}$, where $V_i$'s are subspaces of $V$. It is called the ``sum from $V_1$ up to $V_m$." It is the set of all possible sums of elements of $V_1, \ldots, V_m$, since they all contain the zero-vector.
\end{mydef}

%\textbf{1.40}
\setcounter{thm}{39}
\begin{thm}
  $V_1 + \cdots + V_m$ is the smalles subspace of $V$ containing $V_1, \dots, V_m.$
\end{thm}

\subsection{Direct Sum}

%\textbf{1.41}
\setcounter{thm}{40}
\begin{mydef}[Direct sum]
  \label{def-of-direct-sum}
  %NO COMMA BEFORE IF ACC TO AXLER
  $V_1 + \cdots + V_m$ is called a ``direct sum" if each element of $V_1 +\cdots+V_m$ can be written in only one way as a sum $v_1 + \cdots + v_m$, where each $v_k \in V_k$. In this case we write:
  \begin{equation}
    V_1 \oplus \cdots \oplus V_m :\equiv V_1 + \cdots + V_m
  \end{equation}
\end{mydef}

\begin{example}
  Example: $\myF^3 =
  \left \{ \left ( x, y, 0 \right ) \in \myF^3 \mid x,y \in \myF \right \}
  \oplus
  \left \{ \left (  0, 0, z  \right ) \in \myF^3 \mid z \in \myF \right \}$
\end{example}


%\textbf{1.45}
\setcounter{thm}{44}
\begin{thm} [condition for a direct sum]
  \label{condition-for-a-direct-sum}
  $V_1 + \cdots + V_m$ is a direct sum $\iff$ the only write $0$ as a sum $v_1 + \cdots + v_m$, where each $v_k \in V_k$, is by taking each $v_k$ equal to $0$.
\end{thm}
\begin{proof} Let  $V_1, \ldots, V_m$ be subspaces of $V$ 
  \begin{description}
    \item{$\Rightarrow$ direction:} First suppose $V_1 + \cdots + V_m$ is a direct sum. Let
    \begin{equation}
      0 = v_1 + \cdots + v_m, \whereEach v_k \in V_k
    \end{equation}
    $\implies$ all the $v_k$'s are equal to $0$, because otherwise multiplying the equation above with a scalar $\lambda \in \myF$ would give a different sum
    \begin{equation}
      0 = \lambda0= \lambda v_1 + \cdots + \lambda v_m, \whereEach \lambda v_k \in V_k
    \end{equation}
    Or a different way to argue, $0 = 0 + \cdots + 0$ is already a solution.

    \item{$\Leftarrow$ direction:} Now suppose that the only way to write $0$ as a sum $v_1 + \cdots + v_m$ where each $v_k \in V_k$, is by taking each $v_k = 0$. Let
    \begin{equation}
      \begin{aligned}
        v&=v_1 + \cdots + v_m \where v_1 \in V_1, \ldots, v_m \in V_m \myand \\
        v&=u_1 + \cdots + u_m  \where u_1 \in V_1, \ldots, u_m \in V_m
      \end{aligned}
    \end{equation}
    Subtracting these two equations, we have
    \begin{equation}
      0=(v_1-u_1)+\cdots+(v_m-u_m).
    \end{equation}
    Because $v_1 - u_1 \in V_1, \dots , v_m - u_m \in V_m$, the equation above implies that each $v_k -u_k$ equals $0$.
    \begin{equation}
      \implies v_1=u_1, \ldots, v_m=u_m
    \end{equation}
  \end{description}
\end{proof}

%\textbf{1.46}
\setcounter{thm}{45}
\begin{thm}
  \label{intersection-of-two-direct-sum-of-two-subscpaces}
  $U+W$ is a direct sum $\iff$ $U \cap W = \{0\}$
\end{thm}
\begin{proof}
  \begin{description}
    \item{$\Rightarrow$ direction:} First suppose $U+W$ is a direct sum. If $v \in U \cup W$, then $v, -v \in U \myand v, -v \in W$. We also have that
    \begin{equation}
      0 = v + (-v), \where v\in U \myand (-v) \in W.
    \end{equation}
    $\implies v=0$, because $U+W$  is a direct sum. Therefore $U \cup W = \{0\}$
    \item{$\Leftarrow$ direction:} Suppose $U\cup W = \{0\}$. Let  $u\in U$ and $w \in W$ such that
    \begin{equation}
      0 = u+w
    \end{equation}
    By \ref{condition-for-a-direct-sum} we know that our goal is to show that $u=w=0$. The equation above implies that $u=-w\in W$  and $w=-u \in U$ for all arbitrary choices of $U$ and $W$. Thus $u,w \in U\cup W \implies u=w=0.$ Therefore, $U+W$ is a direct sum.
  \end{description}

\end{proof}
